# substitutions with inequalities

## Example
y=5x-7
-3x-2y=-12

-3x-2(5x-7)=-12
-3x-10x+14=-12
13x+14=-12
    -14-14
    13x=-26
    x=2


    y=5(2)-7
    y=10-7
    y=3

    Answer(2,3)

    There are two y values in this problem. You need to take the equation that has y or x by itself. Then use that equation, and substitute it for x or y in the other problem. Then solve that equation. That is how you get the value of whatever letter you substituted. Now that you know that letter, solve it in the original equationyou used and replace it whith whatever letter you know the value of. Now you have both values. 